pulse/lib/pulse/lib/Pulse.Lib.Slice.fst
@@ -199,7 +199,10 @@ ensures
   with v_dst . assert (pts_to dst v_dst);
   unfold (pts_to dst v_dst);
   unfold (pts_to src #p v);
-  AP.blit src.elt 0sz dst.elt 0sz src.len;
+  AP.memcpy src.elt 0sz dst.elt 0sz src.len;
   fold (pts_to src #p v);
+  assert pure (v `Seq.equal`
+    Seq.append (Seq.slice v 0 (SZ.v src.len))
+      (Seq.slice v_dst (SZ.v src.len) (Seq.length v_dst)));
   fold (pts_to dst v)
 }
